finish casting up to reduction

ArkLib/OracleReduction/Cast.lean
@@ -38,11 +38,23 @@ instance instDCast : DCast Nat ProtocolSpec where
   dcast_id := cast_id
 
 theorem cast_eq_dcast {h : m = n} {pSpec : ProtocolSpec m} :
-    dcast h pSpec = ProtocolSpec.cast h pSpec := rfl
+    pSpec.cast h = dcast h pSpec := rfl
 
 /-! ### Casting (Partial) Transcripts -/
 
-variable {pSpec₁ : ProtocolSpec m} {pSpec₂ : ProtocolSpec n} (hSpec : dcast h pSpec₁ = pSpec₂)
+variable {pSpec₁ : ProtocolSpec m} {pSpec₂ : ProtocolSpec n}
+
+@[simp]
+theorem cast_funext {h} (hSpec : pSpec₁.cast h = pSpec₂) {i : Fin n} :
+    pSpec₁ (Fin.cast h.symm i) = pSpec₂ i := funext_iff.mp hSpec i
+
+alias cast_idx := cast_funext
+
+theorem cast_symm {h} (hSpec : pSpec₁.cast h = pSpec₂) : pSpec₂.cast h.symm = pSpec₁ := by
+  rw [cast_eq_dcast] at hSpec ⊢
+  exact dcast_symm h hSpec
+
+variable (hSpec : pSpec₁.cast h = pSpec₂)
 
 namespace MessageIdx
 
@@ -53,18 +65,44 @@ protected def cast (i : MessageIdx pSpec₁) : MessageIdx pSpec₂ :=
 @[simp]
 theorem cast_id : MessageIdx.cast (Eq.refl m) rfl = (id : pSpec₁.MessageIdx → _) := rfl
 
-instance instDCast : DCast Nat ProtocolSpec where
-  dcast h := ProtocolSpec.cast h
-  dcast_id := cast_id
+instance instDCast₂ : DCast₂ Nat ProtocolSpec (fun _ pSpec => MessageIdx pSpec) where
+  dcast₂ h := MessageIdx.cast h
+  dcast₂_id := cast_id
 
-theorem cast_eq_dcast {h : m = n} {pSpec : ProtocolSpec m} :
-    dcast h pSpec = ProtocolSpec.cast h pSpec := rfl
+theorem cast_eq_dcast₂ {h} {hSpec : pSpec₁.cast h = pSpec₂} {i : MessageIdx pSpec₁}:
+    i.cast h hSpec = dcast₂ h hSpec i := rfl
 
 end MessageIdx
 
+@[simp]
+theorem Message.cast_idx {i : MessageIdx pSpec₂} :
+    pSpec₁.Message (i.cast h.symm (cast_symm hSpec)) = pSpec₂.Message i := by
+  simp [MessageIdx.cast]
+  exact congrArg Prod.snd (cast_funext hSpec)
+
+namespace ChallengeIdx
+
 /-- Casting a challenge index across an equality of `ProtocolSpec`s. -/
-protected def ChallengeIdx.cast (i : ChallengeIdx pSpec₁) : ChallengeIdx pSpec₂ :=
+protected def cast (i : ChallengeIdx pSpec₁) : ChallengeIdx pSpec₂ :=
   ⟨Fin.cast h i.1, by simp [← hSpec, dcast, ProtocolSpec.cast, i.property]⟩
+
+@[simp]
+theorem cast_id : ChallengeIdx.cast (Eq.refl m) rfl = (id : pSpec₁.ChallengeIdx → _) := rfl
+
+instance instDCast₂ : DCast₂ Nat ProtocolSpec (fun _ pSpec => ChallengeIdx pSpec) where
+  dcast₂ h := ChallengeIdx.cast h
+  dcast₂_id := cast_id
+
+theorem cast_eq_dcast₂ {h : m = n} {hSpec : pSpec₁.cast h = pSpec₂} {i : ChallengeIdx pSpec₁}:
+    i.cast h hSpec = dcast₂ h hSpec i := rfl
+
+end ChallengeIdx
+
+@[simp]
+theorem Challenge.cast_idx {i : ChallengeIdx pSpec₂} :
+    pSpec₁.Challenge (i.cast h.symm (cast_symm hSpec)) = pSpec₂.Challenge i := by
+  simp [ChallengeIdx.cast]
+  exact congrArg Prod.snd (cast_funext hSpec)
 
 variable {k : Fin (m + 1)} {l : Fin (n + 1)}
 
@@ -72,7 +110,7 @@ namespace Transcript
 
 /-- Casting two partial transcripts across an equality of `ProtocolSpec`s, where the cutoff indices
   are equal. -/
-protected def cast (hIdx : k.val = l.val) (hSpec : dcast h pSpec₁ = pSpec₂)
+protected def cast (hIdx : k.val = l.val) (hSpec : pSpec₁.cast h = pSpec₂)
     (T : pSpec₁.Transcript k) : pSpec₂.Transcript l :=
   fun i => _root_.cast (by rw [← hSpec]; rfl) (T (Fin.cast hIdx.symm i))
 
@@ -83,13 +121,13 @@ instance instDCast₃ : DCast₃ Nat Fin (fun n _ => ProtocolSpec n)
     (fun _ k pSpec => pSpec.Transcript k) where
   dcast₃ h h' h'' T := Transcript.cast h
     (by simp only [Fin.coe_eq_castSucc, Fin.coe_castSucc]; simp only [dcast] at h'; rw [← h']; rfl)
-    (by simp [← ProtocolSpec.cast_eq_dcast, dcast_eq_root_cast]; exact h'')
+    (by simp [ProtocolSpec.cast_eq_dcast, dcast_eq_root_cast]; exact h'')
     T
   dcast₃_id := cast_id
 
--- theorem cast_eq_dcast₃ (h : m = n) (hIdx : k.val = l.val) (hSpec : dcast h pSpec₁ = pSpec₂)
+-- theorem cast_eq_dcast₃ (h : m = n) (hIdx : k.val = l.val) (hSpec : pSpec₁.cast h = pSpec₂)
 --     (T : Transcript pSpec₁ k) :
---     (dcast₃ h (by sorry) sorry T : pSpec₂.Transcript l) = Transcript.cast h hIdx hSpec T := rfl
+--     T.cast h hIdx hSpec  = (dcast₃ h (by sorry) sorry T : pSpec₂.Transcript l) := rfl
 
 end Transcript
 
@@ -100,7 +138,7 @@ namespace FullTranscript
 /-- Casting a transcript across an equality of `ProtocolSpec`s.
 
 Internally invoke `Transcript.cast` with the last indices. -/
-protected def cast (h : m = n) (hSpec : dcast h pSpec₁ = pSpec₂) (T : FullTranscript pSpec₁) :
+protected def cast (T : FullTranscript pSpec₁) :
     FullTranscript pSpec₂ :=
   Transcript.cast (k := Fin.last m) (l := Fin.last n) h h hSpec T
 
@@ -111,7 +149,7 @@ instance instDCast₂ : DCast₂ Nat ProtocolSpec (fun _ pSpec => FullTranscript
   dcast₂ h h' T := FullTranscript.cast h h' T
   dcast₂_id := cast_id
 
-theorem cast_eq_dcast₂ (h : m = n) (hSpec : dcast h pSpec₁ = pSpec₂) (T : FullTranscript pSpec₁) :
+theorem cast_eq_dcast₂ {T : FullTranscript pSpec₁} :
     dcast₂ h hSpec T = FullTranscript.cast h hSpec T := rfl
 
 end FullTranscript
@@ -120,20 +158,24 @@ end ProtocolSpec
 
 variable {ι : Type} {oSpec : OracleSpec ι} {StmtIn WitIn StmtOut WitOut : Type}
 variable {m n : ℕ} {pSpec₁ : ProtocolSpec m} {pSpec₂ : ProtocolSpec n}
+variable (h : m = n) (hSpec : pSpec₁.cast h = pSpec₂)
+
+open ProtocolSpec
 
 /-! ### Casting Provers -/
 
 namespace Prover
 
 /-- Casting the prover of a non-oracle reduction across an equality of `ProtocolSpec`s. -/
-protected def cast
-    (h : m = n) (hSpec : dcast h pSpec₁ = pSpec₂)
-    (P : Prover oSpec StmtIn WitIn StmtOut WitOut pSpec₁) :
+protected def cast (P : Prover oSpec StmtIn WitIn StmtOut WitOut pSpec₁) :
     Prover oSpec StmtIn WitIn StmtOut WitOut pSpec₂ where
   PrvState := P.PrvState ∘ Fin.cast (congrArg (· + 1) h.symm)
   input := P.input
-  sendMessage := fun i st => P.sendMessage (dcast₂ h hSpec i)
-  receiveChallenge := P.receiveChallenge
+  sendMessage := fun i st => do
+    let ⟨msg, newSt⟩ ← P.sendMessage (i.cast h.symm (cast_symm hSpec)) st
+    return ⟨(Message.cast_idx h hSpec) ▸ msg, newSt⟩
+  receiveChallenge := fun i st chal =>
+    P.receiveChallenge (i.cast h.symm (cast_symm hSpec)) st ((Challenge.cast_idx h hSpec) ▸ chal)
   output := P.output ∘ (fun st => _root_.cast (by simp) st)
 
 end Prover
@@ -145,16 +187,12 @@ namespace Verifier
 /-- Casting the verifier of a non-oracle reduction across an equality of `ProtocolSpec`s.
 
 This boils down to casting the (full) transcript. -/
-protected def cast
-    (h : m = n) (hSpec : dcast h pSpec₁ = pSpec₂)
-    (V : Verifier oSpec StmtIn StmtOut pSpec₁) :
+protected def cast (V : Verifier oSpec StmtIn StmtOut pSpec₁) :
     Verifier oSpec StmtIn StmtOut pSpec₂ where
   verify := fun stmt transcript => V.verify stmt (dcast₂ h.symm (dcast_symm h hSpec) transcript)
 
 @[simp]
-def cast_id
-    (V : Verifier oSpec StmtIn StmtOut pSpec₁) :
-      V.cast rfl rfl = V := by
+theorem cast_id : Verifier.cast rfl rfl = (id : Verifier oSpec StmtIn StmtOut pSpec₁ → _) := by
   ext; simp [Verifier.cast]
 
 instance instDCast₂Verifier :
@@ -162,4 +200,29 @@ instance instDCast₂Verifier :
   dcast₂ := Verifier.cast
   dcast₂_id := by intros; funext; simp
 
+theorem cast_eq_dcast₂ {V : Verifier oSpec StmtIn StmtOut pSpec₁} :
+    V.cast h hSpec = dcast₂ h hSpec V := rfl
+
 end Verifier
+
+namespace Reduction
+
+/-- Casting the reduction of a non-oracle reduction across an equality of `ProtocolSpec`s, which
+  casts the underlying prover and verifier. -/
+protected def cast (R : Reduction oSpec StmtIn WitIn StmtOut WitOut pSpec₁) :
+    Reduction oSpec StmtIn WitIn StmtOut WitOut pSpec₂ where
+  prover := R.prover.cast h hSpec
+  verifier := R.verifier.cast h hSpec
+
+@[simp]
+def cast_id {R : Reduction oSpec StmtIn WitIn StmtOut WitOut pSpec₁} :
+      R.cast rfl rfl = R := by
+  ext : 1 <;> simp [Reduction.cast, Prover.cast, Verifier.cast]
+  rfl
+
+instance instDCast₂Verifier :
+    DCast₂ Nat ProtocolSpec (fun _ pSpec => Verifier oSpec StmtIn StmtOut pSpec) where
+  dcast₂ := Verifier.cast
+  dcast₂_id := by intros; funext; simp
+
+end Reduction
